src/hls/ClockMemoryproof.v
@@ -1,0 +1,500 @@
+(*
+ * Vericert: Verified high-level synthesis.
+ * Copyright (C) 2023 Yann Herklotz <yann@yannherklotz.com>
+ *
+ * This program is free software: you can redistribute it and/or modify
+ * it under the terms of the GNU General Public License as published by
+ * the Free Software Foundation, either version 3 of the License, or
+ * (at your option) any later version.
+ *
+ * This program is distributed in the hope that it will be useful,
+ * but WITHOUT ANY WARRANTY; without even the implied warranty of
+ * MERCHANTABILITY or FITNESS FOR A PARTICULAR PURPOSE.  See the
+ * GNU General Public License for more details.
+ *
+ * You should have received a copy of the GNU General Public License
+ * along with this program.  If not, see <https://www.gnu.org/licenses/>.
+ *)
+
+Require Import Coq.micromega.Lia.
+
+Require Import compcert.backend.Registers.
+Require Import compcert.common.AST.
+Require Import compcert.common.Globalenvs.
+Require compcert.common.Memory.
+Require Import compcert.common.Values.
+Require Import compcert.lib.Floats.
+Require Import compcert.lib.Integers.
+Require Import compcert.lib.Maps.
+Require compcert.common.Smallstep.
+Require compcert.verilog.Op.
+
+Require Import vericert.common.Vericertlib.
+Require Import vericert.hls.ValueInt.
+Require Import vericert.hls.Verilog.
+Require Import vericert.hls.DHTL.
+Require Import vericert.hls.AssocMap.
+Require Import vericert.hls.Array.
+Require Import vericert.hls.DMemorygen.
+Require Import vericert.hls.ClockMemory.
+
+Local Open Scope positive.
+Local Open Scope assocmap.
+
+Inductive match_assocmaps : assocmap -> assocmap -> Prop :=
+  match_assocmap: forall rs rs',
+    (forall r, rs!r = rs'!r) ->
+    match_assocmaps rs rs'.
+
+Inductive match_reg_assocs : reg_associations -> reg_associations -> Prop :=
+  match_reg_association:
+    forall rab rab' ran ran',
+      match_assocmaps rab rab' ->
+      match_assocmaps ran ran' ->
+      match_reg_assocs (mkassociations rab ran) (mkassociations rab' ran').
+
+Inductive match_stackframes : stackframe -> stackframe -> Prop :=
+  match_stackframe_intro :
+    forall r m pc asr asa asr'
+      (MATCH_ASSOC: match_assocmaps asr asr'),
+      match_stackframes (Stackframe r m pc asr asa)
+                        (Stackframe r (transf_module m) pc asr' asa).
+
+Inductive match_states : state -> state -> Prop :=
+| match_state :
+    forall res res' m st asr asr' asa asa'
+           (ASSOC: match_assocmaps asr asr')
+           (ASSOC': match_arrs asa asa')
+           (STACK: Forall2 match_stackframes res res'),
+      match_states (State res m st asr asa)
+                   (State res' (transf_module m) st asr' asa')
+| match_returnstate :
+    forall res res' i
+           (STACKS: Forall2 match_stackframes res res'),
+      match_states (Returnstate res i) (Returnstate res' i)
+| match_initial_call :
+    forall m,
+      match_states (Callstate nil m nil)
+                   (Callstate nil (transf_module m) nil).
+
+Lemma match_assocmaps_refl:
+  forall a, match_assocmaps a a.
+Proof.
+  intros; constructor; auto.
+Qed.
+
+Lemma match_assocmaps_symm:
+  forall a b, match_assocmaps a b -> match_assocmaps b a.
+Proof.
+  inversion 1; constructor; congruence.
+Qed.
+
+Lemma match_assocmaps_trans:
+  forall a b c, match_assocmaps a b -> match_assocmaps b c -> match_assocmaps a c.
+Proof.
+  inversion 1; inversion 1; constructor; congruence.
+Qed.
+
+Lemma match_reg_assocs_trans:
+  forall a b c, match_reg_assocs a b -> match_reg_assocs b c -> match_reg_assocs a c.
+Proof.
+  inversion 1; inversion 1; constructor; subst;
+  eapply match_assocmaps_trans; eauto.
+Qed.
+
+Lemma match_assocs_refl:
+  forall a, match_reg_assocs a a.
+Proof.
+  intros; destruct a; constructor; subst; apply match_assocmaps_refl.
+Qed.
+
+Lemma match_reg_assocs_symm:
+  forall a b, match_reg_assocs a b -> match_reg_assocs b a.
+Proof.
+  inversion 1; constructor; apply match_assocmaps_symm; auto.
+Qed.
+
+Definition match_prog (p: program) (tp: program) :=
+  Linking.match_program (fun cu f tf => tf = transf_fundef f) eq p tp.
+
+Lemma transf_program_match:
+  forall p, match_prog p (transf_program p).
+Proof.
+  intros. unfold transf_program, match_prog.
+  apply Linking.match_transform_program.
+Qed.
+
+Lemma match_assocmaps_inv :
+  forall a b, match_assocmaps a b -> forall x, b ! x = a ! x.
+Proof. inversion 1. auto. Qed.
+
+Lemma match_assocmaps_inv_map :
+  forall a b, match_assocmaps a b -> forall x n, b # (x, n) = a # (x, n).
+Proof. 
+  inversion 1; subst; intros.
+  unfold find_assocmap, AssocMapExt.get_default.
+  now rewrite H0.
+Qed.
+
+Lemma match_assocmaps_merge :
+  forall asr' tasr',
+    match_reg_assocs asr' tasr' ->
+    match_assocmaps (Verilog.merge_regs (assoc_nonblocking asr') (assoc_blocking asr'))
+                          (Verilog.merge_regs (assoc_nonblocking tasr') (assoc_blocking tasr')).
+Proof.
+  inversion 1; subst.
+  inv H0. inv H1. econstructor; intros; cbn.
+  unfold merge_regs. unfold AssocMapExt.merge. rewrite !PTree.gcombine by auto.
+  rewrite H2. now rewrite H0.
+Qed.
+
+Lemma match_assocmaps_merge2 :
+  forall a ta b tb,
+    match_assocmaps a ta ->
+    match_assocmaps b tb ->
+    match_assocmaps (Verilog.merge_regs a b) (Verilog.merge_regs ta tb).
+Proof.
+  inversion 1. inversion 1. subst.
+  econstructor; intros. unfold merge_regs, AssocMapExt.merge.
+  rewrite !PTree.gcombine by auto. rewrite H0. rewrite H4. auto.
+Qed.
+
+Lemma match_assocmaps_set :
+  forall asr asr',
+    match_assocmaps asr asr' ->
+    forall r v, match_assocmaps (AssocMap.set r v asr) (AssocMap.set r v asr').
+Proof.
+  intros. econstructor; intros. destruct (peq r r0); subst.
+  - rewrite !AssocMap.gss; auto.
+  - inv H. rewrite !AssocMap.gso by auto. eauto.
+Qed.
+
+Lemma expr_runp_same :
+  forall f rs1 ar1 c v,
+    expr_runp f rs1 ar1 c v ->
+    forall trs1,
+      match_assocmaps rs1 trs1 ->
+      expr_runp f trs1 ar1 c v.
+Proof.
+  induction 1; intros.
+  - econstructor.
+  - econstructor. erewrite match_assocmaps_inv_map; eauto.
+  - exploit IHexpr_runp; eauto; intros. econstructor; eauto.
+  - exploit IHexpr_runp1; eauto; exploit IHexpr_runp2; eauto; intros.
+    econstructor; eauto.
+  - exploit IHexpr_runp; eauto; intros. econstructor; eauto.
+  - exploit IHexpr_runp1; eauto; exploit IHexpr_runp2; eauto; intros.
+    econstructor; eauto.
+  - exploit IHexpr_runp1; eauto; exploit IHexpr_runp2; eauto; intros.
+    eapply erun_Vternary_false; eauto.
+  - exploit IHexpr_runp; eauto; intros. econstructor; eauto.
+    erewrite match_assocmaps_inv_map; eauto. rewrite H0. now rewrite H1.
+Qed.
+
+Lemma match_states_same :
+  forall f rs1 ar1 c rs2 ar2,
+    stmnt_runp f rs1 ar1 c rs2 ar2 ->
+    forall trs1,
+      match_reg_assocs rs1 trs1 ->
+      exists trs2,
+        stmnt_runp f trs1 ar1 c trs2 ar2
+        /\ match_reg_assocs rs2 trs2.
+Proof.
+  induction 1.
+  - econstructor; split; eauto; constructor.
+  - intros. exploit IHstmnt_runp1; eauto; simplify. 
+    exploit IHstmnt_runp2; eauto; simplify.
+    econstructor; split.
+    + econstructor; eauto.
+    + auto.
+  - intros. exploit IHstmnt_runp; eauto; simplify.
+    inversion H2; subst; exploit expr_runp_same; eauto; intros.
+    eexists; split; eauto; econstructor; eauto.
+  - intros. exploit IHstmnt_runp; eauto; simplify.
+    inversion H2; subst; exploit expr_runp_same; eauto; intros.
+    eexists; split; eauto; eapply stmnt_runp_Vcond_false; eauto.
+  - intros. exploit IHstmnt_runp; eauto; simplify.
+    inversion H3. subst. exploit expr_runp_same; [eapply H| |]; eauto; intros.
+    exploit expr_runp_same; [eapply H0| |]; eauto; intros.
+    eexists; split; eauto. econstructor; eauto.
+  - intros. exploit IHstmnt_runp; eauto; simplify.
+    inversion H3. subst. exploit expr_runp_same; [eapply H| |]; eauto; intros.
+    exploit expr_runp_same; [eapply H0| |]; eauto; intros.
+    eexists; split; eauto. eapply stmnt_runp_Vcase_match; eauto.
+  - intros. exploit IHstmnt_runp; eauto; simplify.
+    inversion H1. subst. exploit expr_runp_same; [eapply H| |]; eauto; intros.
+    eexists; split; eauto. eapply stmnt_runp_Vcase_default; eauto.
+  - inv H; intros.
+    inversion H. subst. exploit expr_runp_same; eauto; intros.
+    econstructor; split; intros. econstructor; eauto. econstructor.
+    econstructor; cbn; eauto.
+    econstructor; intros.
+    destruct (peq r r0); subst.
+    + now rewrite !AssocMap.gss.
+    + rewrite !AssocMap.gso by auto. inv H1; eauto.
+  - inv H; intros.
+    inversion H. subst. exploit expr_runp_same; eauto; intros.
+    econstructor; split; intros. econstructor; eauto. econstructor.
+    econstructor; cbn; eauto.
+    econstructor; intros.
+    destruct (peq r r0); subst.
+    + now rewrite !AssocMap.gss.
+    + rewrite !AssocMap.gso by auto. inv H2; eauto.
+  - inv H; intros. inversion H; subst.
+    exploit expr_runp_same; [eapply H0| |]; eauto; intros.
+    exploit expr_runp_same; [eapply H6| |]; eauto; intros.
+    eexists; split; eauto. econstructor; eauto. econstructor; eauto.
+  - inv H; intros. inversion H; subst.
+    exploit expr_runp_same; [eapply H0| |]; eauto; intros.
+    exploit expr_runp_same; [eapply H6| |]; eauto; intros.
+    eexists; split; eauto. econstructor; eauto. econstructor; eauto.
+Qed.
+
+Lemma exec_ram_same :
+  forall rs1 ar1 c rs2 ar2,
+    exec_ram rs1 ar1 c rs2 ar2 ->
+    forall trs1,
+      match_reg_assocs rs1 trs1 ->
+      exists trs2,
+        exec_ram trs1 ar1 c trs2 ar2
+        /\ match_reg_assocs rs2 trs2.
+Proof.
+  induction 1; intros.
+  - eexists; split; eauto.
+    apply exec_ram_Some_idle. inv H0. cbn in *; setoid_rewrite match_assocmaps_inv_map; eauto.
+  - inv H6; eexists; split; cbn in *.
+    + eapply exec_ram_Some_write. eapply H. eauto. all: cbn in *.
+      now erewrite match_assocmaps_inv_map by eauto.
+      all: now erewrite match_assocmaps_inv by eauto.
+    + unfold nonblock_reg; cbn. constructor; auto.
+      now apply match_assocmaps_set.
+  - inv H5; eexists; split; cbn in *.
+    + eapply exec_ram_Some_read; eauto; cbn in *.
+      now erewrite match_assocmaps_inv_map by eauto.
+      all: now erewrite match_assocmaps_inv by eauto.
+    + unfold nonblock_reg; cbn. constructor; auto.
+      now repeat apply match_assocmaps_set.
+  - eexists; split; cbn in *; eauto. econstructor.
+Qed.
+
+  Lemma expr_interchangeable:
+    forall e r v a ar f v',
+      check_excluded r e = true ->
+      expr_runp f a ar e v ->
+      expr_runp f (AssocMap.set r v' a) ar e v.
+  Proof. 
+    induction e; intros; cbn in *; simplify; try rewrite negb_true_iff in *;
+    repeat match goal with | H: _ =? _ = false |- _ => apply Pos.eqb_neq in H end; inv H0; try solve [econstructor; eauto].
+    - econstructor; now rewrite assocmap_gso by auto.
+    - econstructor; eauto; now rewrite assocmap_gso by auto.
+  Qed.
+
+  Lemma expr_interchangeable2:
+    forall e r v a ar f v',
+      check_excluded r e = true ->
+      expr_runp f (AssocMap.set r v' a) ar e v ->
+      expr_runp f a ar e v.
+  Proof. 
+    induction e; intros; cbn in *; simplify; try rewrite negb_true_iff in *;
+    repeat match goal with | H: _ =? _ = false |- _ => apply Pos.eqb_neq in H end; inv H0; try solve [econstructor; eauto].
+    - econstructor; now rewrite assocmap_gso by auto.
+    - econstructor; eauto; now rewrite assocmap_gso by auto.
+  Qed.
+
+  Lemma expr_interchangeable3:
+    forall e r t asr iv v arr v',
+      check_excluded r e = true ->
+      expr_runp t asr (arr_assocmap_set r (valueToNat iv) v arr) e v' ->
+      expr_runp t asr arr e v'.
+  Proof.
+    induction e; intros; cbn in *; simplify; try rewrite negb_true_iff in *;
+    repeat match goal with | H: _ =? _ = false |- _ => apply Pos.eqb_neq in H end; inv H0; try solve [econstructor; eauto].
+    econstructor; eauto. unfold arr_assocmap_lookup in *. unfold arr_assocmap_set in *.
+    destruct (arr ! r0) eqn:?; auto. rewrite AssocMap.gso in H9 by auto. auto.
+  Qed.
+
+  Lemma transf_maps_correct:
+    forall t asr asa s asr' asa',
+      stmnt_runp t (mkassociations asr empty_assocmap) asa s asr' asa' ->
+      (forall r e1 e0 r0 e3, s <> (Vseq (Vseq Vskip (Vblock (Vvari r e1) e0)) (Vblock (Vvar r0) e3))) ->
+      forall tasr,
+        match_reg_assocs (mkassociations asr empty_assocmap) (mkassociations tasr empty_assocmap) ->
+        exists tasr', stmnt_runp t (mkassociations tasr empty_assocmap) asa (transf_maps s) tasr' asa'
+                      /\ match_assocmaps (Verilog.merge_regs (assoc_nonblocking asr') (assoc_blocking asr'))
+                      (Verilog.merge_regs (assoc_nonblocking tasr') (assoc_blocking tasr')).
+  Proof.
+    intros * ? HNEQ **. destruct s; try solve [exploit match_states_same; eauto; simplify;
+      exploit match_assocmaps_merge; eauto].
+    cbn in *. 
+    repeat (destruct_match; try solve [exploit match_states_same; eauto; simplify;
+      exploit match_assocmaps_merge; eauto]).
+    - simplify.
+      inv H. inv H11. inv H10. inv H14; inv H10. inv H15; inv H10.
+      inv H14.
+      eexists; split. econstructor. econstructor. econstructor.
+      2: { econstructor. econstructor. econstructor. unfold block_reg in *; cbn in *. eapply expr_interchangeable; eauto.
+           eapply expr_runp_same; eauto. inv H0; auto. eauto. }
+      unfold block_reg in *; cbn in *. eapply expr_interchangeable2; eauto.
+      eapply expr_runp_same; eauto. eapply match_assocmaps_set; eauto.
+      inv H0; auto.
+      econstructor; intros. cbn.
+      unfold merge_regs, AssocMapExt.merge. inv H0; subst; cbn.
+      rewrite !PTree.gcombine by auto.
+      rewrite negb_true_iff in *.
+      apply Pos.eqb_neq in H4. apply Pos.eqb_neq in H2. apply Pos.eqb_neq in H5.
+      destruct (peq r r2); subst.
+      + rewrite !AssocMap.gss by auto. rewrite !AssocMap.gso by auto. auto.
+      + rewrite !AssocMap.gso by auto.
+        destruct (peq r r1); subst.
+        ** rewrite !AssocMap.gss. rewrite !AssocMap.gso by auto. auto.
+        ** rewrite !AssocMap.gso by auto. inv H8. rewrite H. auto.
+    - subst. exfalso; eapply HNEQ; eauto.
+  Qed.
+
+  Lemma transf_maps_correct2:
+    forall t asr asa s asr' asa',
+      stmnt_runp t (mkassociations asr empty_assocmap) asa s asr' asa' ->
+      (forall r e1 e0 r0 e3, s <> (Vseq (Vseq Vskip (Vblock (Vvari r e1) e0)) (Vblock (Vvar r0) e3))) ->
+      forall tasr,
+        match_reg_assocs (mkassociations asr empty_assocmap) (mkassociations tasr empty_assocmap) ->
+        exists tasr', stmnt_runp t (mkassociations tasr empty_assocmap) asa (transf_maps s) tasr' asa'
+                      /\ match_assocmaps (Verilog.merge_regs (assoc_nonblocking asr') (assoc_blocking asr'))
+                      (Verilog.merge_regs (assoc_nonblocking tasr') (assoc_blocking tasr')).
+  Proof.
+
+  Lemma transf_maps_correct2:
+    forall t asr asa r e1 e0 r0 e3 asr' asa' st l,
+      stmnt_runp t (mkassociations asr empty_assocmap) (mkassociations asa (empty_stack st l)) 
+        (Vseq (Vseq Vskip (Vblock (Vvari r e1) e0)) (Vblock (Vvar r0) e3)) asr' asa' ->
+      forall tasr,
+        match_reg_assocs (mkassociations asr empty_assocmap) (mkassociations tasr empty_assocmap) ->
+        exists tasr' tasa', stmnt_runp t (mkassociations tasr empty_assocmap) (mkassociations asa (empty_stack st l)) 
+                        (transf_maps (Vseq (Vseq Vskip (Vblock (Vvari r e1) e0)) (Vblock (Vvar r0) e3))) tasr' tasa'
+                      /\ match_assocmaps (Verilog.merge_regs (assoc_nonblocking asr') (assoc_blocking asr'))
+                      (Verilog.merge_regs (assoc_nonblocking tasr') (assoc_blocking tasr'))
+                      /\ Verilog.merge_arrs (assoc_nonblocking tasa') (assoc_blocking tasa') 
+                         = Verilog.merge_arrs (assoc_nonblocking asa') (assoc_blocking asa').
+  Proof.
+    intros; cbn in *. inv H0. clear H6.
+    inv H. inv H6. inv H5. inv H9; inv H5. inv H10; inv H5. cbn in *. destruct_match; cbn in *;
+    repeat (kill_bools; match goal with | H: _ /\ _ |- _ => inv H end).
+    - rewrite negb_true_iff in *. apply Pos.eqb_neq in H0. do 2 eexists; split; [|split].
+      + econstructor. econstructor. econstructor. cbn. eapply expr_interchangeable3; eauto.
+        eapply expr_runp_same; eauto.
+        eapply stmnt_runp_Vnonblock_arr. econstructor. 
+        cbn. eapply expr_interchangeable; eauto. eapply expr_runp_same; eauto.
+        cbn. eapply expr_interchangeable; eauto. eapply expr_runp_same; eauto.
+      + cbn. eapply match_assocmaps_merge2; eauto. apply match_assocmaps_refl.
+        now apply match_assocmaps_set.
+      + cbn. unfold merge_arrs.
+
+Section CORRECTNESS.
+
+  Context (prog tprog: program).
+  Context (TRANSL: match_prog prog tprog).
+
+  Let ge : genv := Genv.globalenv prog.
+  Let tge : genv := Genv.globalenv tprog.
+
+  Lemma symbols_preserved:
+    forall (s: AST.ident), Genv.find_symbol tge s = Genv.find_symbol ge s.
+  Proof using TRANSL. intros. eapply (Genv.find_symbol_match TRANSL). Qed.
+  #[local] Hint Resolve symbols_preserved : mgen.
+
+  Lemma function_ptr_translated:
+    forall (b: Values.block) (f: fundef),
+      Genv.find_funct_ptr ge b = Some f ->
+      exists tf,
+        Genv.find_funct_ptr tge b = Some tf /\ transf_fundef f = tf.
+  Proof using TRANSL.
+    intros. exploit (Genv.find_funct_ptr_match TRANSL); eauto.
+    intros (cu & tf & P & Q & R); exists tf; auto.
+  Qed.
+  #[local] Hint Resolve function_ptr_translated : mgen.
+
+  Lemma functions_translated:
+    forall (v: Values.val) (f: fundef),
+      Genv.find_funct ge v = Some f ->
+      exists tf,
+        Genv.find_funct tge v = Some tf /\ transf_fundef f = tf.
+  Proof using TRANSL.
+    intros. exploit (Genv.find_funct_match TRANSL); eauto.
+    intros (cu & tf & P & Q & R); exists tf; auto.
+  Qed.
+  #[local] Hint Resolve functions_translated : mgen.
+
+  Lemma senv_preserved:
+    Senv.equiv (Genv.to_senv ge) (Genv.to_senv tge).
+  Proof (Genv.senv_transf TRANSL).
+  #[local] Hint Resolve senv_preserved : mgen.
+
+  Theorem transf_step_correct:
+    forall (S1 : state) t S2,
+      step ge S1 t S2 ->
+      forall R1,
+        match_states S1 R1 ->
+        exists R2, step tge R1 t R2 /\ match_states S2 R2.
+  Proof. 
+    induction 1.
+    - inversion 1; subst. exploit transf_maps_correct; eauto. econstructor. eauto.
+      apply match_assocmaps_refl. intros ((btasr' & ntasr') & HSTMNT & HMATCH).
+      exploit exec_ram_same; eauto. econstructor; eauto. apply match_assocmaps_refl.
+      intros ((btrs2 & ntrs2) & HEXEC & HMATCH2).
+      econstructor. split. econstructor; cbn.
+      1-3: now erewrite match_assocmaps_inv by eauto.
+      rewrite PTree.gmap1. rewrite H2. cbn. auto. eassumption.
+      eassumption. eauto. eauto. eapply match_assocmaps_merge in HMATCH2.
+      erewrite match_assocmaps_inv; eauto. eauto.
+      econstructor; auto. eapply match_assocmaps_merge in HMATCH2. eauto.
+    - inversion 1; subst. econstructor; split.
+      apply step_finish; cbn. now erewrite match_assocmaps_inv by eauto.
+      erewrite match_assocmaps_inv by eauto. eassumption.
+      econstructor; auto.
+    - inversion 1; subst; intros. econstructor; split.
+      apply step_call. econstructor; auto. inv H.
+      repeat apply match_assocmaps_set. cbn. 
+      apply match_assocmaps_refl.
+    - inversion 1; subst. inv STACKS. inv H0. destruct y.  
+      eexists; split. eapply step_return. eauto. inv H2.
+      constructor; auto. repeat apply match_assocmaps_set. auto.
+  Qed.
+  #[local] Hint Resolve transf_step_correct : mgen.
+
+  Lemma transf_initial_states :
+    forall s1 : state,
+      initial_state prog s1 ->
+      exists s2 : state,
+        initial_state tprog s2 /\ match_states s1 s2.
+  Proof using TRANSL.
+    simplify. inv H.
+    exploit function_ptr_translated. eauto. intros.
+    inv H. inv H3.
+    econstructor. econstructor. econstructor.
+    eapply (Genv.init_mem_match TRANSL); eauto.
+    setoid_rewrite (Linking.match_program_main TRANSL).
+    rewrite symbols_preserved. eauto.
+    eauto.
+    econstructor.
+  Qed.
+  #[local] Hint Resolve transf_initial_states : mgen.
+
+  Lemma transf_final_states :
+    forall (s1 : state)
+           (s2 : state)
+           (r : Int.int),
+      match_states s1 s2 ->
+      final_state s1 r ->
+      final_state s2 r.
+  Proof using TRANSL.
+    intros. inv H0. inv H. inv STACKS. unfold valueToInt. constructor. auto.
+  Qed.
+  #[local] Hint Resolve transf_final_states : mgen.
+
+  Theorem transf_program_correct:
+    Smallstep.forward_simulation (semantics prog) (semantics tprog).
+  Proof using TRANSL.
+    eapply Smallstep.forward_simulation_step; eauto with mgen.
+    apply senv_preserved. intros. eapply transf_final_states; eauto.
+  Qed.
+
+End CORRECTNESS.
